theories/examples/proofs_enc.v
@@ -10,7 +10,7 @@ Section ExampleProofsEnc.
   Context `{!heapG Σ} (N : namespace).
   Context `{!logrelG val Σ}.
 
-  Notation "⟦ c @ s : sτ ⟧{ γ }" := (interp_st N γ (stype'_to_stype sτ) c s)
+  Notation "⟦ c @ s : sτ ⟧{ γ }" := (interp_st N γ (lift_stype sτ) c s)
     (at level 10, s at next level, sτ at next level, γ at next level,
      format "⟦  c  @  s  :  sτ  ⟧{ γ }").
 
@@ -20,7 +20,7 @@ Section ExampleProofsEnc.
     iIntros (Φ H) "HΦ".
     rewrite /seq_example.
     wp_apply (new_chan_st_enc_spec N
-             (TSR' Send (λ v, ⌜v = 5⌝%I) (λ v, TEnd')))=> //;
+             (TSR Send (λ v, ⌜v = 5⌝%I) (λ v, TEnd)))=> //;
     iIntros (c γ) "[Hstl Hstr]"=> /=.
     wp_apply (send_st_enc_spec N Z with "[$Hstl //]");
     iIntros "Hstl".
@@ -39,11 +39,11 @@ Section ExampleProofsEnc.
     iIntros (Φ H) "HΦ".
     rewrite /par_2_example.
     wp_apply (new_chan_st_enc_spec N
-      (TSR' Send
+      (TSR Send
            (λ v:Z, ⌜5 ≤ v⌝%I)
-           (λ v:Z, TSR' Receive
+           (λ v:Z, TSR Receive
                      (λ v':Z, ⌜v+2 ≤ v'⌝%I)
-                     (λ v':Z, TEnd'))))=> //;
+                     (λ v':Z, TEnd))))=> //;
     iIntros (c γ) "[Hstl Hstr]"=> /=.
     wp_apply (wp_fork with "[Hstr]").
     - iNext.
@@ -67,8 +67,8 @@ Section ExampleProofsEnc.
     iIntros (Φ H) "HΦ".
     rewrite /heaplet_example.
     wp_apply (new_chan_st_enc_spec N
-      (TSR' Send (λ v, (v ↦ #5)%I)
-                (λ v, TEnd')))=> //;
+      (TSR Send (λ v, (v ↦ #5)%I)
+                (λ v, TEnd)))=> //;
     iIntros (c γ) "[Hstl Hstr]"=> /=.
     wp_apply (wp_fork with "[Hstl]").
     - iNext.
@@ -89,16 +89,16 @@ Section ExampleProofsEnc.
     iIntros (Φ H) "HΦ".
     rewrite /channel_example.
     wp_apply (new_chan_st_enc_spec N
-      (TSR' Send (λ v, ∃ γ, ⟦ v @ Right :
-        (TSR' Receive
+      (TSR Send (λ v, ∃ γ, ⟦ v @ Right :
+        (TSR Receive
              (λ v, ⌜v = 5⌝)
-             (λ _, TEnd')) ⟧{γ})%I
-                (λ v, TEnd')))=> //;
+             (λ _, TEnd)) ⟧{γ})%I
+                (λ v, TEnd)))=> //;
     iIntros (c γ) "[Hstl Hstr]"=> /=.
     wp_apply (wp_fork with "[Hstl]").
     - iNext.
       wp_apply (new_chan_st_enc_spec N
-        (TSR' Send (λ v, ⌜v = 5⌝%I) (λ v, TEnd')))=> //;
+        (TSR Send (λ v, ⌜v = 5⌝%I) (λ v, TEnd)))=> //;
       iIntros (c' γ') "[Hstl' Hstr']"=> /=.
       wp_apply (send_st_enc_spec N val with "[Hstl Hstr']");
         first by eauto 10 with iFrame.
